@prefix owl: <http://www.w3.org/2002/07/owl#> .
@prefix rdf: <http://www.w3.org/1999/02/22-rdf-syntax-ns#> .
@prefix rdfs: <http://www.w3.org/2000/01/rdf-schema#> .
@prefix s223: <http://data.ashrae.org/standard223#> .
@prefix sh: <http://www.w3.org/ns/shacl#> .
@prefix xsd: <http://www.w3.org/2001/XMLSchema#> .
@prefix watr: <urn:nawi-water-ontology#> .

<urn:nawi-water-ontology/equip>
    a owl:Ontology ;
    rdfs:label "NAWI Water Equipment Ontology" ;
    rdfs:comment "An ontology for water equipment used in the NAWI project" ;
    owl:imports <http://data.ashrae.org/standard223/1.0/model/all> ;
.
watr:Tank a rdfs:Class, sh:NodeShape ;
    rdfs:label "Tank" ;
    rdfs:comment "A tank for storing liquid" ;
    rdfs:subClassOf s223:Equipment ;
    sh:property [
        sh:path s223:hasConnectionPoint ;
        rdfs:comment "A tank has an inlet fluid connection point" ;
        sh:qualifiedMinCount 1 ;
        sh:qualifiedValueShape [
            sh:class s223:InletConnectionPoint ;
            sh:property [
                sh:path s223:hasMedium ;
                sh:hasValue s223:Mix-Fluid ;
            ] ;
        ] ;
    ] ;
    sh:property [
        sh:path s223:hasConnectionPoint ;
        rdfs:comment "A tank has an outlet fluid connection point" ;
        sh:qualifiedMinCount 1 ;
        sh:qualifiedValueShape [
            sh:class s223:OutletConnectionPoint ;
            sh:property [
                sh:path s223:hasMedium ;
                sh:hasValue s223:Mix-Fluid ;
            ] ;
        ] ;
    ] ;
.

watr:Reactor
    rdfs:label "Reactor" ;
    rdfs:comment "An equipment used for chemical reaction" ;
    rdfs:subClassOf watr:Tank ;
    sh:property [
        sh:path s223:hasConnectionPoint ;
        rdfs:comment "A reactor has at least one inlet fluid connection point" ;
        sh:qualifiedMinCount 1 ;
        sh:qualifiedValueShape [
            sh:class s223:InletConnectionPoint ;
            sh:property [
                sh:path s223:hasMedium ;
                sh:hasValue s223:Mix-Fluid ;
            ] ;
        ] ;
    ] ;
    sh:property [
        sh:path s223:hasConnectionPoint ;
        rdfs:comment "A reactor has at least one outlet fluid connection point" ;
        sh:qualifiedMinCount 1 ;
        sh:qualifiedValueShape [
            sh:class s223:OutletConnectionPoint ;
            sh:property [
                sh:path s223:hasMedium ;
                sh:hasValue s223:Mix-Fluid ;
            ] ;
        ] ;
    ] ;
.

watr:SequencingBatchReactor
    rdfs:label "SequencingBatchReactor" ;
    rdfs:comment "A type of activated sludge process for wastewater treatment" ;
    rdfs:subClassOf watr:Reactor .

watr:PlugFlowReactor
    rdfs:label "PlugFlowReactor" ;
    rdfs:comment "A type of reactor where the fluid flows in one direction through the tube" ;
    rdfs:subClassOf watr:Reactor .

watr:ContinuouslyStirredTankReactor
    rdfs:label "ContinuouslyStirredTankReactor" ;
    rdfs:comment "A reactor in which contents are well mixed and reactants are added continuously" ;
    rdfs:subClassOf watr:Reactor .

watr:StaticMixer
    rdfs:label "StaticMixer" ;
    rdfs:comment "A device for mixing liquids without moving components" ;
    rdfs:subClassOf watr:Reactor .

watr:AerationBasin
    rdfs:label "AerationBasin" ;
    rdfs:comment "A tank where water is aerated to remove gases and volatile organic compounds" ;
    rdfs:subClassOf watr:Reactor .

watr:Digester
    rdfs:label "Digester" ;
    rdfs:comment "A container to promote decomposition of organic waste" ;
    rdfs:subClassOf watr:Tank .
watr:AnaerobicDigester
    rdfs:label "AnaerobicDigester" ;
    rdfs:comment "A container to promote decomposition of organic waste in anaerobic conditions" ;
    rdfs:subClassOf watr:Digester .
watr:AerobicDigester
    rdfs:label "AerobicDigester" ;
    rdfs:comment "A container to promote decomposition of organic waste in aerobic conditions" ;
    rdfs:subClassOf watr:Digester .

watr:DisinfectionUnit
    rdfs:label "Disinfection" ;
    rdfs:comment "A unit used to eliminate or reduce harmful microorganisms" ;
    rdfs:subClassOf watr:Tank .

watr:UltravioletLightUnit
    rdfs:label "UltravioletlightUnit" ;
    rdfs:comment "A unit using ultraviolet light for disinfection" ;
    rdfs:subClassOf watr:DisinfectionUnit .

watr:ChlorinationBasin
    rdfs:label "ChlorinationBasin" ;
    rdfs:comment "A basin where chlorine is added for disinfection" ;
    rdfs:subClassOf watr:DisinfectionUnit .

watr:SedimentationTank
    rdfs:label "SedimentationTank" ;
    rdfs:comment "A tank used to remove solids from liquids through sedimentation" ;
    rdfs:subClassOf watr:Tank .

watr:Screen
    rdfs:label "Screen" ;
    rdfs:comment "An equipment used for separation" ;
    rdfs:subClassOf s223:Equipment .

watr:GritChamber
    rdfs:label "Grit Chamber" ;
    rdfs:comment "A chamber used to remove grit from wastewater" ;
    rdfs:subClassOf s223:Equipment .

watr:Reservoir
    rdfs:label "Reservoir" ;
    rdfs:comment "A large natural or artificial body of water used for water supply" ;
    rdfs:subClassOf s223:Equipment .

watr:Pond
    rdfs:label "Pond" ;
    rdfs:comment "A body of still water smaller than a lake, used for treatment or storage" ;
    rdfs:subClassOf s223:Equipment .

watr:Battery
    rdfs:label "Battery" ;
    rdfs:comment "A device that stores energy for later use" ;
    rdfs:subClassOf s223:Battery .

watr:Cogenerator
    rdfs:label "Cogenerator" ;
    rdfs:comment "An equipment that produces both electricity and heat from the same energy source" ;
    rdfs:subClassOf s223:Equipment .

watr:Boiler
    rdfs:label "Boiler" ;
    rdfs:comment "A device for heating water" ;
    rdfs:subClassOf s223:Boiler .

watr:Conditioner
    rdfs:label "Conditioner" ;
    rdfs:comment "An equipment used to prepare raw biogas from a digester by removing impurities" ;
    rdfs:subClassOf s223:Equipment .

watr:Flare
    rdfs:label "Flare" ;
    rdfs:comment "A device used to burn off unwanted gas" ;
    rdfs:subClassOf s223:Equipment .

watr:Pump
    rdfs:label "Pump" ;
    rdfs:comment "A device used to move fluids by mechanical action" ;
    rdfs:subClassOf s223:Pump .

watr:PressureExchanger
    rdfs:label "PressureExchanger" ;
    rdfs:comment "A device used to transfer pressure energy from one fluid to another" ;
    rdfs:subClassOf s223:Equipment .

watr:DewateringUnit
    rdfs:label "Dewatering" ;
    rdfs:comment "A unit used to remove water from solid material" ;
    rdfs:subClassOf s223:Equipment .

watr:Thickener
    rdfs:label "Thickener" ;
    rdfs:comment "A device used to increase the solids concentration of a slurry" ;
    rdfs:subClassOf s223:Equipment .

watr:DissolvedAirFlotationThickener
    rdfs:label "DissolvedAirFlotationThickener" ;
    rdfs:comment "A thickener that uses dissolved air to separate solids from liquids" ;
    rdfs:subClassOf watr:Thickener .

watr:CentrifugalThickener
    rdfs:label "CentrifugalThickener" ;
    rdfs:comment "A thickener that uses centrifugal force to separate solids from liquids" ;
    rdfs:subClassOf watr:Thickener .

watr:GravityThickener
    rdfs:label "GravityThickener" ;
    rdfs:comment "A thickener that uses gravity to separate solids from liquids" ;
    rdfs:subClassOf watr:Thickener .

watr:BeltThickener
    rdfs:label "BeltThickener" ;
    rdfs:comment "A thickener that uses a belt system to separate solids from liquids" ;
    rdfs:subClassOf watr:Thickener .

watr:GravityBeltThickener
    rdfs:label "Gravity Belt Thickener" ;
    rdfs:comment "A thickener that combines gravity separation with a belt system" ;
    rdfs:subClassOf watr:BeltThickener .

watr:RotaryDrumThickener
    rdfs:label "Rotary Drum Thickener" ;
    rdfs:comment "A thickener that uses a rotating drum to separate solids from liquids" ;
    rdfs:subClassOf watr:Thickener .

watr:Filter
    rdfs:label "Filter" ;
    rdfs:comment "An equipment used to remove impurities from liquids or gases" ;
    rdfs:subClassOf s223:Filter .

watr:ReverseOsmosisMembrane
    rdfs:label "ReverseOsmosisMembrane" ;
    rdfs:comment "A membrane used for reverse osmosis" ;
    rdfs:subClassOf watr:Filter .
    
watr:ReverseOsmosisMembrane
    rdfs:label "ReverseOsmosisMembrane" ;
    rdfs:comment "A membrane used for reverse osmosis" ;
    rdfs:subClassOf watr:Filter .

watr:TricklingFilter
    rdfs:label "TricklingFilter" ;
    rdfs:comment "A filter system that treats wastewater by trickling it over a bed of rocks or plastic" ;
    rdfs:subClassOf watr:Filter .

watr:MembraneBioreactor
    rdfs:label "MembraneBioreactor" ;
    rdfs:comment "A filter system that combines a membrane process like microfiltration with a biological reactor" ;
    rdfs:subClassOf watr:Filter .

watr:MicrofiltrationUnit
    rdfs:label "MicrofiltrationUnit" ;
    rdfs:comment "A filter system which removes contaminants from a liquid by passing it through a microporous membrane" ;
    rdfs:subClassOf watr:Filter .

watr:UltrafiltrationUnit
    rdfs:label "UltrafiltrationUnit" ;
    rdfs:comment "A filter system that uses a pressure-driven barrier to separate particles and solutes in a fluid" ;
    rdfs:subClassOf watr:Filter .

watr:NanofiltrationUnit
    rdfs:label "NanofiltrationUnit" ;
    rdfs:comment "A filter system that uses a membrane to soften water and remove organic contaminants" ;
    rdfs:subClassOf watr:Filter .

watr:MediaFiltration
    rdfs:label "MediaFiltrationUnit" ;
    rdfs:comment "A filter system that uses a bed of material to filter out contaminants" ;
    rdfs:subClassOf watr:Filter .

watr:CartridgeFiltrationUnit
    rdfs:label "CartridgeFiltrationUnit" ;
    rdfs:comment "A filter system using a cartridge to remove contaminants from fluids" ;
    rdfs:subClassOf watr:Filter .
    
watr:IonExchangeMembrane
    rdfs:label "IonExchangeMembrane" ;
    rdfs:comment "A membrane that selectively allows ions to pass through while blocking other substances" ;
    rdfs:subClassOf s223:Equipment .

watr:ElectrodialysisUnit
    rdfs:label "Electrodialysis" ;
    rdfs:comment "A unit that uses electricity to drive ion movement through a membrane" ;
    rdfs:subClassOf s223:Equipment .

watr:Electrolyzer
    rdfs:label "Electrolyzer" ;
    rdfs:comment "An equipment that uses electricity to split liquids into constituent elements" ;
    rdfs:subClassOf s223:Equipment .

watr:Crystallizer
    rdfs:label "Crystallizer" ;
    rdfs:comment "An equipment used to produce solid crystals from a solution" ;
    rdfs:subClassOf s223:Equipment .

watr:Compressor
    rdfs:label "Compressor" ;
    rdfs:comment "An equipment that increases the pressure of a gas" ;
    rdfs:subClassOf s223:Compressor .

watr:Evaporator
    rdfs:label "Evaporator" ;
    rdfs:comment "A device used to turn the liquid form of a substance into its gaseous form" ;
    rdfs:subClassOf s223:HeatExchanger .

watr:Condenser
    rdfs:label "Condenser" ;
    rdfs:comment "A device used to condense a gaseous substance back into a liquid" ;
    rdfs:subClassOf s223:HeatExchanger .

watr:FlowSensor
    rdfs:label "FlowSensor" ;
    rdfs:comment "A sensor used to measure the flow rate of liquids or gases" ;
    rdfs:subClassOf s223:FlowSensor .

watr:VolumeSensor
    rdfs:label "VolumeSensor" ;
    rdfs:comment "A sensor used to measure the volume of a substance" ;
    rdfs:subClassOf s223:Sensor .

watr:LevelSensor
    rdfs:label "LevelSensor" ;
    rdfs:comment "A sensor used to detect the level of liquids or solids in a tank" ;
    rdfs:subClassOf s223:Sensor .

watr:PressureSensor
    rdfs:label "PressureSensor" ;
    rdfs:comment "A sensor used to measure pressure" ;
    rdfs:subClassOf s223:PressureSensor .

watr:TemperatureSensor
    rdfs:label "TemperatureSensor" ;
    rdfs:comment "A sensor used to measure temperature" ;
    rdfs:subClassOf s223:TemperatureSensor .

watr:ConcentrationSensor
    rdfs:label "ConcentrationSensor" ;
    rdfs:comment "A sensor used to measure the concentration of specific substances (e.g., Total Dissolved Solids)" ;
    rdfs:subClassOf s223:ConcentrationSensor .

watr:OxygenMeter
    rdfs:label "Oxygen Meter" ;
    rdfs:comment "A sensor used to measure the concentration of oxygen" ;
    rdfs:subClassOf s223:ConcentrationSensor .

watr:OxygenDemandSensor
    rdfs:label "OxygenDemandSensor" ;
    rdfs:comment "A sensor used to measure Chemical Oxygen Demand (COD) and Biological Oxygen Demand (BOD)" ;
    rdfs:subClassOf s223:Sensor .

watr:pHSensor
    rdfs:label "pHSensor" ;
    rdfs:comment "A sensor used to measure the pH of a solution" ;
    rdfs:subClassOf watr:ConcentrationSensor .

watr:ConductivitySensor
    rdfs:label "ConductivitySensor" ;
    rdfs:comment "A sensor used to measure the electrical conductivity of a solution" ;
    rdfs:subClassOf watr:Sensor .

watr:TurbidityMeter
    rdfs:label "TurbidityMeter" ;
    rdfs:comment "A sensor used to measure the turbidity (clarity) of a fluid" ;
    rdfs:subClassOf watr:Sensor .

watr:RotationSensor
    rdfs:label "RotationSensor" ;
    rdfs:comment "A sensor used to measure the rotational speed or position of an object" ;
    rdfs:subClassOf s223:Sensor .

watr:EfficiencySensor
    rdfs:label "EfficiencySensor" ;
    rdfs:comment "A sensor used to measure the efficiency of a system or equipment" ;
    rdfs:subClassOf s223:Sensor .

watr:StateOfChargeSensor
    rdfs:label "State of Charge Sensor" ;
    rdfs:comment "A sensor used to measure the remaining charge in a battery or energy storage system" ;
    rdfs:subClassOf s223:Sensor .

watr:SpeedSensor
    rdfs:label "Speed Sensor" ;
    rdfs:comment "A sensor used to measure the speed of an object or fluid" ;
    rdfs:subClassOf s223:Sensor .

watr:FrequencySensor
    rdfs:label "Frequency Sensor" ;
    rdfs:comment "A sensor used to measure the frequency of a signal or mechanical vibration" ;
    rdfs:subClassOf s223:Sensor .

# Do we want something like this? Is modeling a TOC sensor without explicitly naming it too vague (Concentration sensor, measuring organics)
watr:TotalOrganicCompoundConcentrationSensor
    rdfs:label "TOC Sensor" ;
    rdfs:comment "A sensor used to measure the total organic compound concentration" ;
    rdfs:subClassOf watr:ConcentrationSensor ;
.
# I just forgot this one originally I think
watr:Membrane
    a s223:Class ;
    rdfs:subClassOf s223:Filter 
.
watr:Valve 
    a s223:Class; 
    rdfs:subClassOf s223:Valve 
.
watr:VariableFrequencyDrive
    a s223:Class ;
    rdfs:subClassOf s223:VariableFrequencyDrive
.
watr:ThreeWayValve 
    a s223:Class; 
    rdfs:subClassOf s223:Valve 
.
watr:CheckValve
    a s223:Class; 
    rdfs:subClassOf s223:Valve
.
watr:Controller 
    a s223:Class ;
    rdfs:subClassOf s223:Controller ;
.
watr:ManualMeasurementPort 
    rdfs:label "Manual Measurement Port" ;
    rdfs:comment "A location where manual measurements are taken" ;
    rdfs:subClassOf s223:Sensor ;
.
# Runtime can just be an enumeration kind - these are just properties
# watr:RunTimeSensor
#     rdfs:label "RunTimeSensor" ;
#     rdfs:comment "A sensor used to measure the operating time of equipment" ;
#     rdfs:subClassOf s223:Sensor .

# watr:RunStatusSensor
#     rdfs:label "RunStatusSensor" ;
#     rdfs:comment "A sensor used to monitor the operational status of equipment" ;
#     rdfs:subClassOf s223:Sensor .
